\documentclass{article}
\usepackage[utf8]{inputenc}
\usepackage{amsmath, enumerate, multicol}
\usepackage[margin = 0.5in]{geometry}
\pagestyle{empty}
\raggedright
\everymath{\displaystyle}
\newcounter{PS}


\begin{document}

Name \makebox[3in]{\hrulefill} \hfill Honors PreCalc PSet

\subsubsection*{Function Operations \hfill \makebox[0.35in]{\hrulefill} / 10}

Use the pair of functions $f$ and $g$ to find the following values if they exist. \newline\\

\begin{tabular}{p{0.2\textwidth}p{0.2\textwidth}p{0.2\textwidth}p{0.2\textwidth}}
    \textbullet $(f+g)(2)$  &
    \textbullet $(f-g)(-1)$ &
    \textbullet $(fg)\left(\frac{1}{2}\right)$ &
    \textbullet $\left(\frac{f}{g}\right)(0)$   \\
\end{tabular}
\begin{multicols}{3}
\begin{enumerate}
    \item $f(x) = x^2-x$ and $g(x) = 12-x^2$
    \item $f(x) = \sqrt{x+3}$ and $g(x) = 2x-1$
    \item $f(x) = x^2$ and $g(x) = \frac{3}{2x-3}$
\setcounter{PS}{\value{enumi}}
\end{enumerate}
\end{multicols}
\vfill

Use the pair of functions $f$ and $g$ to simplify each expression. \textbf{Then state its domain}.  \newline\\

\begin{tabular}{p{0.2\textwidth}p{0.2\textwidth}p{0.2\textwidth}p{0.2\textwidth}}
    \textbullet $(f+g)(x)$  &
    \textbullet $(f-g)(x)$ &
    \textbullet $(fg)(x)$ &
    \textbullet $\left(\frac{f}{g}\right)(x)$   \\
\end{tabular}

\begin{multicols}{2}
\begin{enumerate}   \setcounter{enumi}{\value{PS}}
    \item $f(x) = 2x+1$ and $g(x) = x-2$
    \item $f(x) = x^2$ and $g(x) = 3x-1$
\setcounter{PS}{\value{enumi}}
\end{enumerate}
\end{multicols}
\vfill
\begin{multicols}{2}
\begin{enumerate}   \setcounter{enumi}{\value{PS}}
    \item $f(x) = \frac{x}{2}$ and $g(x) = \frac{2}{x}$
    \item $f(x) = x$ and $g(x) = \sqrt{x+1}$
\setcounter{PS}{\value{enumi}}
\end{enumerate}
\end{multicols}
\vfill
\newpage

Name \makebox[3in]{\hrulefill} \hfill Honors PreCalc Function Operations PSet   \newline\\
Find the difference quotient for each.
\begin{multicols}{2}
\begin{enumerate}   \setcounter{enumi}{\value{PS}}
    \item $f(x) = 2x-5$
    \item $f(x) = 6$
\setcounter{PS}{\value{enumi}}
\end{enumerate}
\end{multicols}
\vfill
\begin{multicols}{2}
\begin{enumerate}   \setcounter{enumi}{\value{PS}}
    \item $f(x) = 3x^2-x$
    \item $f(x) = \frac{2}{x}$
\end{enumerate}
\end{multicols}
\vfill

\newpage

\textsc{Function Operations KEY}

\begin{enumerate}   \setlength{\itemsep}{15pt}
\begin{multicols}{3}
    \item 
    \begin{itemize}
        \item $(f+g)(2) = 10$
        \item $(f-g)(-1) = -9$
        \item $(fg)\left(\frac{1}{2}\right) = -\frac{47}{16}$
        \item $\left(\frac{f}{g}\right)(0) = 0$
    \end{itemize}
    \item
    \begin{itemize}
        \item $(f+g)(2) = 3+\sqrt{5}$
        \item $(f-g)(-1) = 3+\sqrt{2}$
        \item $(fg)\left(\frac{1}{2}\right) = 0$
        \item $\left(\frac{f}{g}\right)(0) = -\sqrt{3}$
    \end{itemize}
    \item
    \begin{itemize}
        \item $(f+g)(2) = 7$
        \item $(f-g)(-1) = \frac{8}{5}$
        \item $(fg)\left(\frac{1}{2}\right) = -\frac{3}{8}$
        \item $\left(\frac{f}{g}\right)(0) = 0$
    \end{itemize}
\end{multicols}
\vspace{0.25in}
    \item 
    \begin{itemize}
        \item $(f+g)(x)=3x-1$ \quad Domain: $(-\infty, \infty)$
        \item $(f-g)(x)=x+3$ \quad Domain: $(-\infty, \infty)$
        \item $(fg)(x)=2x^2-3x-2$ \quad Domain: $(-\infty, \infty)$
        \item $\left(\frac{f}{g}\right)(x)=\frac{2x+1}{x-2}$ \quad Domain: $(-\infty,2)\cup (2,\infty)$
    \end{itemize}
    \item 
    \begin{itemize}
        \item $(f+g)(x)=x^2+3x-1$ \quad Domain: $(-\infty, \infty)$
        \item $(f-g)(x)=x^2-3x+1$ \quad Domain: $(-\infty, \infty)$
        \item $(fg)(x)=3x^3-x^2$ \quad Domain: $(-\infty, \infty)$
        \item $\left(\frac{f}{g}\right)(x)=\frac{x^2}{3x-1}$ \quad Domain: $\left(-\infty,\frac{1}{3}\right) cup \left(\frac{1}{3},\infty\right)$
    \end{itemize}
    \item
    \begin{itemize}
        \item $(f+g)(x)=\frac{x^2+4}{2x}$ \quad Domain: $(-\infty, 0) \cup (0,\infty)$
        \item $(f-g)(x)=\frac{x^2-4}{2x}$ \quad Domain: $(-\infty, 0) \cup (0,\infty)$
        \item $(fg)(x)=1$ \quad Domain: $(-\infty, 0) \cup (0,\infty)$
        \item $\left(\frac{f}{g}\right)(x)=\frac{x^2}{4}$ \quad Domain: $(-\infty, 0) \cup (0,\infty)$
    \end{itemize}
    \item
    \begin{itemize}
        \item $(f+g)(x)=x+\sqrt{x+1}$ \quad Domain: $[-1,\infty)$
        \item $(f-g)(x)=x-\sqrt{x+1}$ \quad Domain: $[-1,\infty)$
        \item $(fg)(x)=x\sqrt{x+1}$ \quad Domain: $[-1,\infty)$
        \item $\left(\frac{f}{g}\right)(x)=\frac{x}{\sqrt{x+1}}$ \quad Domain: $(-1,\infty)$
    \end{itemize}
\vspace{0.25in}
    \begin{multicols}{4}
    \item 2
    \item 0
    \item $6x+3h-1$
    \item $\frac{-2}{x(x+h)}$
    \end{multicols}
\end{enumerate}
\end{document}
