\documentclass{article}
\usepackage{amsmath}
\usepackage[margin=0.5in]{geometry}
\pagestyle{empty}
\raggedright
\everymath{\displaystyle}

\begin{document}

Name \makebox[3in]{\hrulefill} \hfill Honors PreCalc P-Set

\subsubsection*{Polynomials and Their Graphs \hfill \makebox[0.35in]{\hrulefill} / 10}

Determine whether each is a polynomial.
\begin{flalign*}
1.	\quad	&	f(x) = 3x^4 - 6x^2 + x^{-1}	&
2.	\quad	&	g(x) = -2x^3 - 7x^5 + 4			&
3.	\quad	&	h(x) = |4x|								&&\\[0.5in]
\end{flalign*}

Determine the degree, leading term, leading coefficient, and constant term of each.
\begin{flalign*}
4.	\quad	&	f(x) = 4 - x - 3x^2					&
5.	\quad	&	g(x) = 3x^5 - 2x^2 + x + 1		&
6.	\quad	&	Z(b) = 42b - b^3					&&\\[1.25in]
7. \quad	&	f(x) = \sqrt{3}x^{17} + 22.5x^{10}-\pi x^7 + \frac{1}{3}	&
8.	\quad	&	P(x) = (x-1)(x-2)(x-3)(x-4)		&
9.	\quad	&	f(x) = -2x^3(x+1)(x+2)^2		&&\\[1.25in]
\end{flalign*}

Determine the end behavior of each.
\begin{flalign*}
10.	\quad	&	f(x) = 4 - x - 3x^2					&
11.	\quad	&	g(x) = 3x^5 - 2x^2 + x + 1		&
12.	\quad	&	Z(b) = 42b - b^3					&&\\[1in]
13. 	\quad	&	f(x) = \sqrt{3}x^{17} + 22.5x^{10}-\pi x^7 + \frac{1}{3}	&
14.	\quad	&	P(x) = (x-1)(x-2)(x-3)(x-4)		&
15.	\quad	&	f(x) = -2x^3(x+1)(x+2)^2		&&\\[1in]
\end{flalign*}

Find the zeros of each.
\begin{flalign*}
16.	\quad	&	a(x) = x^3 + 4x^2 + 4x					&
17.	\quad	&	g(x) = 4x^3 - 8x^2 - 11x - 3				&
18.	\quad	&	Q(x) = (x+5)^2(x-3)^4			&&\\
\end{flalign*}
\newpage

\textsc{Key}
\begin{enumerate}
	\item Not a polynomial
	\item Is a polynomial
	\item Not a polynomial
	\item degree = 2, leading term = $-3x^2$, leading coefficient = $-3$ constant = 4
	\item degree = 5, leading term = $3x^5$, leading coefficient = 3, constant = 1
	\item degree = 3, leading term = $-b^3$, leading coefficient = $-1$, constant = 0
	\item degree = 17, leading term = $\sqrt{3}x^{17}$, leading coefficient = $\sqrt{3}$, constant = $\frac{1}{3}$
	\item degree = 4, leading term = $x^4$, leading coefficient = 1, constant = 24
	\item degree = 6, leading term = $-2x^6$, leading coefficient = $-2$, constant = 0
	\item $\lim_{x\to -\infty}f(x) = -\infty \quad \lim_{x\to \infty}f(x) = -\infty$
	\item $\lim_{x\to -\infty}g(x) = -\infty \quad \lim_{x\to \infty}g(x) = \infty$
	\item $\lim_{b\to -\infty}Z(b) = \infty \quad \lim_{b\to \infty}Z(b) = -\infty$
	\item $\lim_{x\to -\infty}f(x) = -\infty \quad \lim_{x\to \infty}f(x) = \infty$
	\item $\lim_{x\to -\infty}P(x) = \infty \quad \lim_{x\to \infty}P(x) = \infty$
	\item $\lim_{x\to -\infty}f(x) = -\infty \quad \lim_{x\to \infty}f(x) = -\infty$
	\item $x = -2, 0$
	\item $x = -\frac{1}{2}, 3$
	\item $x = -5, 3$
\end{enumerate}

\end{document}
